Define terminal object through graphs

coq/Graph.v
@@ -466,3 +466,27 @@ Section GraphExtension.
 
 End GraphExtension.
 
+Section GraphTerminal.
+  Context {C : PreCategory}.
+
+  Definition TerminalGr : Graph C 0 0.
+  Proof. srapply mkGraph; inv_fin_0'. Defined.
+  Definition Terminal := Limit TerminalGr.
+  Definition term_obj (T : Terminal) := cn_top (lim_cone T).
+
+  Definition term_cone (c : object C) : Cone TerminalGr.
+  Proof. srapply mkCone; [ exact c | inv_fin_0' | inv_fin_0' ]. Defined.
+  Lemma terminal_ex (c : object C) (T : Terminal) : morphism C c (term_obj T).
+  Proof. exact (cnmph_mph (lim_ex T (term_cone c))). Qed.
+
+  Definition term_mph {c1 : object C} (c2 : Cone TerminalGr) (f : morphism C c1 (cn_top c2)) :
+    ConeMorphism (term_cone c1) c2.
+  Proof. srapply mkCnMph; [ exact f | inv_fin_0' ]. Defined.
+  Lemma terminal_uniq (c : object C) (T : Terminal) :
+    forall(f g : morphism C c (term_obj T)), f = g.
+  Proof.
+    intros f g. pose (f' := term_mph (lim_cone T) f). pose (g' := term_mph (lim_cone T) g).
+    exact (lim_uniq T _ f' g').
+  Qed.
+
+End GraphTerminal.
